changed test.fs to add marshalling

ModularEngine/src/LogicEngine.FStar/test.fs
@@ -2,14 +2,15 @@ module Test
 
 exception Error of string
 
-let sendMsg (p:string) (msg:string) =
+let sendMsg (me:string) (p:string) (msg:string) =
   let bytes = System.Text.Encoding.Unicode.GetBytes msg in
-  let _ = Net.send p bytes in
+  let _ = Net.sendForTest me p bytes in
   System.Console.WriteLine("sent " + msg)
 
 let getMsg() =
   let bytes = Net.receive() in
-  let msg = System.Text.Encoding.Unicode.GetString(bytes) in
+  let bys = Net.recvForTest bytes in
+  let msg = System.Text.Encoding.Unicode.GetString(bys) in
   System.Console.WriteLine("got " + msg)
 
 let _ = 
@@ -21,11 +22,11 @@ let _ =
       else Authenticate.readConfig configFile
     | _ -> (System.Console.WriteLine("usage: test config-file-name"); exit(1)) in
   let p = Authenticate.lookup_me() in
-  if (p = "org1") then sendMsg "site1" "msg from org1 to site1"
+  if (p = "org1") then sendMsg "org1" "site1" "msg from org1 to site1"
   else if (p = "site1") then
-    (getMsg(); sendMsg "phys1" "msg from site1 to phys1")
+    (getMsg(); sendMsg "site1" "phys1" "msg from site1 to phys1")
   else if (p = "phys1") then
-    (getMsg(); sendMsg "keyMgr" "msg from phys1 to keyMgr"; getMsg(); Prims.stopAllServers true; ())
+    (getMsg(); sendMsg "phys1" "keyMgr" "msg from phys1 to keyMgr"; getMsg(); Prims.stopAllServers true; ())
   else if (p = "keyMgr") then
-    (getMsg(); sendMsg "phys1" "msg keys from keyMgr to phys1")
+    (getMsg(); sendMsg "keyMgr" "phys1" "msg keys from keyMgr to phys1")
     
